\documentclass[letterpaper]{report}

\setlength\parindent{0pt}
\usepackage[utf8]{inputenc}
\usepackage[T1]{fontenc}
\usepackage{textcomp}
\usepackage{amsmath, amssymb}
\usepackage{enumitem}
\title{Weekly HW 3}
\author{Svadrut Kukunooru}
\date{\today}

\begin{document}
\begin{titlepage}
    \maketitle
\end{titlepage}

\subsection{Section 1.6, Problem 10}%
\label{sub:Section 1.6, Problem 10}
In the following problem, let $f : \mathbb{R}^7 \to \mathbb{R}^3$ for the matrix transformation defined by $f(x) = Ax$, where 
\[
A = 
\begin{bmatrix} 
    1 & 2 \\
    0 & 1 \\
    1 & 1
\end{bmatrix} 
\] 
Determine whether the matrix $w = \begin{bmatrix} 
1 \\ 1 \\ 1
\end{bmatrix}$ is in the range of $f$.
\[
\begin{bmatrix} 
    1 & 2 \\
    0 & 1 \\
    1 & 1
\end{bmatrix} 
\begin{bmatrix} 
x \\ y
\end{bmatrix} = 
\begin{bmatrix} 
1 \\ 1 \\ 1
\end{bmatrix} 
\] 
\begin{equation}
    \begin{cases}
        x + 2y = 1 \\
        y = 1 \\
        x + y = 1
    \end{cases}
\end{equation}
Since this system of equations is impossible to solve, \fbox{the matrix $w$ is NOT in the range of $f$.}

\subsection{Section 2.1, Problem 6}%
\label{sub:Section 2.1, Problem 6}
Find the reduced row echelon form of each of the given matrices. Record the row operations you perform, using the notation for elementary row operations. 
        \[
        \begin{bmatrix}
            -1 & 2 & -5 \\
            2 & -1 & 6 \\
            2 & -2 & 7
        \end{bmatrix}
   \] 
\[
\begin{bmatrix} 
    -1 & 2 & -5 \\
    0 & 3 & -4 \\
    2 & -2 & 7
\end{bmatrix} \to (R_3 + 2R_1 = R_3, -R_1 = R_1) \to
\begin{bmatrix} 
    1 & -2 & 5 \\
    0 & 3 & -4 \\
    0 & 2 & -3
\end{bmatrix} 
\] 
\[
\begin{bmatrix} 
    1 & -2 & 5 \\
    0 & 3 & -4 \\
    0 & 2 & -3
\end{bmatrix} 
\to (R_2 - R_3= R_2) \to 
\begin{bmatrix} 
    1 & -2 & 5 \\
    0 & 1 & -1 \\
    0 & 2 & -3
\end{bmatrix} 
\] 
\[
\begin{bmatrix} 
    1 & -2 & 5 \\
    0 & 1 & -1 \\
    0 & 2 & -3
\end{bmatrix} \to 
(R_3 - 2R_2 = R_3) \to
\begin{bmatrix} 
    1 & -2 & 5 \\
    0 & 1 & -1 \\
    0 & 0 & -1
\end{bmatrix}
\] 
\[
\begin{bmatrix} 
    1 & -2 & 5 \\
    0 & 1 & -1 \\
    0 & 0 & -1
\end{bmatrix}
\to (R_1 + 2R_2= R_1) \to 
\begin{bmatrix} 
    1 & 0 & 3 \\
    0 & 1 & -1 \\
    0 & 0 & -1  
\end{bmatrix} 
\] 
\[
\begin{bmatrix} 
    1 & 0 & 3 \\
    0 & 1 & -1 \\
    0 & 0 & -1
\end{bmatrix} \to (-R_3 = R_3) \to 
\begin{bmatrix} 
    1 & 0 & 3 \\
    0 & 1 & -1 \\
    0 & 0 & 1
\end{bmatrix} 
\] 
\[
\begin{bmatrix} 
    1 & 0 & 3 \\
    0 & 1 & -1 \\
    0 & 0 & 1
\end{bmatrix} \to (R_2 + R_3 = R_2) \to 
\begin{bmatrix} 
    1 & 0 & 3 \\
    0 & 1 & 0 \\
    0 & 0 & 1
\end{bmatrix} 
\] 
\[
\begin{bmatrix} 
    1 & 0 & 3 \\
    0 & 1 & 0 \\
    0 & 0 & 1
\end{bmatrix} \to 
(R_1 - 3R_3 = R_1) \to
\fbox{$
\begin{bmatrix} 
    1 & 0 & 0 \\
    0 & 1 & 0 \\
    0 & 0 & 1
\end{bmatrix} = I_3 $}
\] 
\noindent\makebox[\linewidth]{\rule{\linewidth}{0.4pt}}
    \[
    \begin{bmatrix} 
        1 & 1 & -1 \\
        3 & 4 & -1 \\
        5 & 6 & 3 \\
        -2 & -2 & 2
    \end{bmatrix} 
    \] 
\[
\begin{bmatrix} 
        1 & 1 & -1 \\
        3 & 4 & -1 \\
        5 & 6 & 3 \\
        -2 & -2 & 2
    \end{bmatrix}
\to (R_2 - 3R_1 = R_2, R_3 - 5R_1 = R_3, R_4 + 2R_1 = R_4) \to 
\begin{bmatrix} 
    1 & 1 & -1 \\
    0 & 1 & 2 \\
    0 & 1 & 8 \\
    0 & 0 & 0 
\end{bmatrix} 
\]
\[ 
\begin{bmatrix} 
    1 & 1 & -1 \\
    0 & 1 & 2 \\
    0 & 1 & 8 \\
    0 & 0 & 0 
\end{bmatrix} 
    \to (R_1 - R_2 = R_1, R_3-R_2 = R_3) \to  
\begin{bmatrix} 
    1 & 0 & -3 \\
    0 & 1 & 2 \\
    0 & 0 & 6 \\
    0 & 0 & 0
\end{bmatrix} 
\] 
\[
\begin{bmatrix} 
    1 & 0 & -3 \\
    0 & 1 & 2 \\
    0 & 0 & 6 \\
    0 & 0 & 0
\end{bmatrix} 
    \to (R_3 \times \frac{1}{6} = R_3) \to 
    \begin{bmatrix} 
        1 & 0 & -3 \\
        0 & 1 & 2 \\
        0 & 0 & 1 \\
        0 & 0 & 0
    \end{bmatrix} 
\] 
\[
    \begin{bmatrix} 
        1 & 0 & -3 \\
        0 & 1 & 2 \\
        0 & 0 & 1 \\
        0 & 0 & 0
    \end{bmatrix} 
    \to (R_2 - 2R_3 = R_2, R_1 + 3R_3 = R_1) \to 
    \fbox{$
    \begin{bmatrix} 
        1 & 0 & 0 \\
        0 & 1 & 0 \\
        0 & 0 & 1 \\
        0 & 0 & 0
\end{bmatrix} $}
\] 
\subsection{Section 2.2, Problem 9}%
\label{sub:Section 2.2, Problem 9}
In this exercise, solve the linear system, with the given augmented matrix, if it is consistent.
\[
\begin{bmatrix} 
    1 & 2 & 1 & | & 7 \\
    2 & 0 & 1 & | & 4 \\
    1 & 0 & 2 & | & 5 \\
    1 & 2 & 3 & | & 11 \\
    2 & 1 & 4 & | & 12 
\end{bmatrix} 
\]
\[
\begin{bmatrix} 
    1 & 2 & 1 & | & 7 \\
    2 & 0 & 1 & | & 4 \\
    1 & 0 & 2 & | & 5 \\
    1 & 2 & 3 & | & 11 \\
    2 & 1 & 4 & | & 12 
\end{bmatrix} \to 
(R_2 - 2R_1 = R_2, R_3 - R_1 = R_3, R_4 - R_1 = R_4, R_5 - 2R_1 = R_5) \to \]\[ \to
\begin{bmatrix} 
    1 & 2 & 1 & | & 7 \\
    0 & -4 & -1 & | & -10 \\ 
    0 & -2 & 1 & | & -2 \\
    0 & 0 & 2 & | & 4 \\
    0 & -3 & 2 & | & -2
\end{bmatrix} \to  (R_2 - R_5 = R_2) \to 
\begin{bmatrix} 
    1 & 2 & 1 & | & 7 \\
    0 & -1 & -3 & | & -8 \\
    0 & -2 & 1 & | & -2 \\
    0 & 0 & 2 & | & 4 \\
    0 & -3 & 2 & | & -2
\end{bmatrix} \to 
\] 
\[
\begin{bmatrix} 
    1 & 2 & 1 & | & 7 \\
    0 & -1 & -3 & | & -8 \\
    0 & -2 & 1 & | & -2 \\
    0 & 0 & 2 & | & 4 \\
    0 & -3 & 2 & | & -2
\end{bmatrix} 
\to (-R_2 = R_2) \to 
\begin{bmatrix} 
    1 & 2 & 1 & | & 7 \\
    0 & 1 & 3 & | & 8 \\
    0 & -2 & 1 & | & -2 \\
    0 & 0 & 2 & | & 4 \\
    0 & -3 & 2 & | & -2
\end{bmatrix} 
\]

I don't really have to simplify the augmented matrix anymore, now that I know that $2z = 4$. Therefore, $z = 2$.
Using the third line, I conclude that $y = 2$. Testing this with the other equations, this substitution of $z=2$ and $y=2$ yields no inconsistency. Substituting both of these into the first line yields $x$ as 1. 
\[
    \fbox{$x=1,y=2,z=2$}
\] 
\noindent\makebox[\linewidth]{\rule{\linewidth}{0.4pt}}
\[
\begin{bmatrix} 
    1 & 2 & 1 & | & 0 \\
    2 & 3 & 0 & | & 0 \\
    0 & 1 & 2 & | & 0 \\
    2 & 1 & 4 & | & 0
\end{bmatrix} 
\] There is a trivial solution, but I'll attempt to find another solution using row operations and RREFs. 
\[
\begin{bmatrix} 
    1 & 2 & 1 & | & 0 \\
    2 & 3 & 0 & | & 0 \\
    0 & 1 & 2 & | & 0 \\
    2 & 1 & 4 & | & 0
\end{bmatrix} \to 
(R_2 - 2R_1 = R_2, R_4 - 2R_1 = R_4) \to 
\begin{bmatrix} 
    1 & 2 & 1 & | & 0 \\
    0 & -1 & -2 & | & 0 \\
    0 & 1 & 2 & | & 0 \\
    0 & -3 & 2 & | & 0
\end{bmatrix} 
\]
I don't need to simplify anymore, because I see that there is an inconsistency; both $1y + 2z$ and $-3y + 2z$ are equal to zero, making the system of equations inconsistent. There is only the trivial solution. 
\[
    \fbox{$x=0,y=0,z=0$}
\] 
\end{document}
